theories/examples/cmdc/cmdc.v
@@ -1,0 +1,88 @@
+From iris.algebra Require Import frac.
+From iris.proofmode Require Import proofmode.
+From cap_machine Require Import rules proofmode.
+From cap_machine Require Import fetch assert.
+
+Section CMDC_Main.
+  Context `{MP: MachineParameters}.
+
+  (* Expect:
+     pc := (RX, Global, b_main, e_main, b_main_code )
+
+     b_main + 0 : WCap E_XSRW_ b_switcher e_switcher a_cc_switcher
+     b_main + 1 : WCap E_RX b_assert e_assert a_assert
+     b_main + 2 : WSealed ot_switcher B.f
+     b_main + 3 : WSealed ot_switcher C.g
+
+   *)
+  Definition cmdc_main_code : list Word :=
+    encodeInstrsW [
+      (* #"main_b_code"; *)
+
+      (* set b <- 0 *)
+      Store cgp 0%Z;
+      Mov ca0 cgp;
+
+      (* set c <- 0 *)
+      Lea cgp 1%Z;
+      Store cgp 0%Z;
+
+      (* call B.f b *)
+      GetA ct0 ca0;
+      Add ct1 ct0 1%Z;
+      Subseg ca0 ct0 ct1 (* ca0 -> b *)
+    ]
+    ++ fetch_instrs 0 ctp ct0 ct1 (* ctp -> switcher entry point *)
+    ++ fetch_instrs 2 cs0 ct0 ct1 (* cs0 -> {B.f}_(ot_switcher)  *)
+    ++
+    encodeInstrsW [
+      Jalr cra ctp;
+      (* assert c == 0 *)
+      Load ct0 cgp; (* ct0 -> c *)
+      Mov ct1 0%Z
+    ]
+    ++ assert_instrs 1 ct2 ct3 ct4 (* asserts that ( *ct0 = *ct1 ) *)
+    ++
+    encodeInstrsW [
+      (* prepare for later *)
+      Mov ca0 cgp;
+      Mov ca1 0%Z; (* erase returned values from the call *)
+
+      (* set b <- 42 *)
+      Lea cgp (-1)%Z;
+      Store cgp 42%Z;
+
+      (* call C.g c *)
+      GetA ct0 ca0;
+      Add ct1 ct0 1%Z;
+      Subseg ca0 ct0 ct1 (* ca0 -> c *)
+    ]
+    ++ fetch_instrs 0 ctp ct0 ct1 (* ctp -> switcher entry point *)
+    ++ fetch_instrs 3 cs0 ct0 ct1 (* cs0 -> {C.g}_(ot_switcher)  *)
+    ++
+    encodeInstrsW [
+      Jalr cra ctp;
+      (* assert b == 42 *)
+      Load ct0 cgp; (* ct0 -> c *)
+      Mov ct1 42%Z
+    ]
+    ++ assert_instrs 1 ct2 ct3 ct4 (* asserts that ( *ct0 = *ct1 ) *)
+    ++ encodeInstrsW [
+      Halt
+      (* #"main_e" *)
+    ].
+
+  Definition cmdc_main_data : list Word := [WInt 0; WInt 0].
+
+  Definition cmdc_main_imports
+    (b_switcher e_switcher a_cc_switcher : Addr) (ot_switcher : OType)
+    (b_assert e_assert : Addr)
+    (B_f C_g : Sealable) : list Word :=
+    [
+      WCap E_XSRW_ Global b_switcher e_switcher a_cc_switcher;
+      WCap E_RX Global b_assert e_assert b_assert;
+      WSealed ot_switcher B_f;
+      WSealed ot_switcher C_g
+    ].
+
+End CMDC_Main.
