theories/examples/cmdc/cmdc_adequacy.v
@@ -1,0 +1,708 @@
+From iris.proofmode Require Import proofmode.
+From cap_machine Require Import logrel.
+From cap_machine Require Import compartment_layout.
+From cap_machine Require Import cmdc cmdc_spec.
+From cap_machine Require Import switcher switcher_spec assert logrel.
+From cap_machine Require Import mkregion_helpers.
+From cap_machine Require Import region_invariants_allocation.
+From iris.program_logic Require Import adequacy.
+From iris.base_logic Require Import invariants.
+
+Class memory_layout `{MachineParameters} := {
+
+    (* switcher *)
+    switcher_cmpt : cmptSwitcher;
+
+    (* assert *)
+    assert_cmpt : cmptAssert;
+
+    (* main compartment *)
+    main_cmpt : cmpt ;
+
+    (* adv compartments B and C *)
+    B_cmpt : cmpt ;
+    C_cmpt : cmpt ;
+
+    (* disjointness *)
+    cmpts_disjoints :
+    main_cmpt ## B_cmpt
+    ∧ main_cmpt ## C_cmpt
+    ∧ B_cmpt ## C_cmpt ;
+
+    switcher_cmpt_disjoints :
+    switcher_cmpt_disjoint main_cmpt switcher_cmpt
+    ∧ switcher_cmpt_disjoint B_cmpt switcher_cmpt
+    ∧ switcher_cmpt_disjoint C_cmpt switcher_cmpt ;
+
+    assert_cmpt_disjoints :
+    assert_cmpt_disjoint main_cmpt assert_cmpt
+    ∧ assert_cmpt_disjoint B_cmpt assert_cmpt
+    ∧ assert_cmpt_disjoint C_cmpt assert_cmpt ;
+
+    assert_switcher_disjoints :
+    assert_switcher_disjoint assert_cmpt switcher_cmpt;
+  }.
+
+Definition mk_initial_memory `{memory_layout} (mem: Mem) :=
+  mk_initial_switcher switcher_cmpt ∪
+    mk_initial_assert assert_cmpt ∪
+    mk_initial_cmpt main_cmpt ∪
+    mk_initial_cmpt B_cmpt ∪
+    mk_initial_cmpt C_cmpt.
+
+
+Definition is_initial_registers `{memory_layout} (reg: Reg) :=
+  reg !! PC = Some (WCap RX Global (cmpt_b_pcc main_cmpt) (cmpt_e_pcc main_cmpt) (cmpt_a_code main_cmpt)) ∧
+  reg !! cgp = Some (WCap RW Global (cmpt_b_cgp main_cmpt) (cmpt_e_cgp main_cmpt) (cmpt_b_cgp main_cmpt)) ∧
+  reg !! csp = Some (WCap RWL Local (b_stack switcher_cmpt) (e_stack switcher_cmpt) (b_stack switcher_cmpt)) ∧
+  (∀ (r: RegName), r ∉ ({[ PC; cgp; csp ]} : gset RegName) → reg !! r = Some (WInt 0)).
+
+Definition is_initial_sregisters `{memory_layout} (sreg : SReg) :=
+  sreg !! MTDC = Some (WCap RWL Local
+                         (b_trusted_stack switcher_cmpt)
+                         (e_trusted_stack switcher_cmpt)
+                         (b_trusted_stack switcher_cmpt)).
+
+Definition is_initial_memory `{memory_layout} (mem: Mem) :=
+  let switcher_entry :=
+    WCap E_XSRW_ Global
+      (b_switcher switcher_cmpt)
+      (e_switcher switcher_cmpt)
+      (a_switcher_cc switcher_cmpt)
+  in
+  let B_f :=
+    SCap RO Global
+      (cmpt_exp_tbl_pcc B_cmpt)
+      (cmpt_exp_tbl_entries_end B_cmpt)
+      (cmpt_exp_tbl_entries_start B_cmpt)
+  in
+  let C_g :=
+    SCap RO Global
+      (cmpt_exp_tbl_pcc C_cmpt)
+      (cmpt_exp_tbl_entries_end C_cmpt)
+      (cmpt_exp_tbl_entries_start C_cmpt)
+  in
+
+  mem = mk_initial_memory mem
+  (* instantiating main *)
+  ∧ (cmpt_imports main_cmpt) =
+    cmdc_main_imports
+      (b_switcher switcher_cmpt) (e_switcher switcher_cmpt)
+      (a_switcher_cc switcher_cmpt) (ot_switcher switcher_cmpt)
+      (b_assert assert_cmpt) (e_assert assert_cmpt)
+      B_f C_g
+  ∧ (cmpt_code main_cmpt) = cmdc_main_code
+  ∧ (cmpt_data main_cmpt) = cmdc_main_data
+  ∧ (cmpt_exp_tbl_entries main_cmpt) = []
+
+  (* instantiating B *)
+  ∧ (cmpt_imports B_cmpt) = [switcher_entry]
+  ∧ Forall is_z (cmpt_code B_cmpt) (* only instructions *)
+  ∧ Forall is_z (cmpt_data B_cmpt) (* TODO generalise: either z or in_region *)
+  ∧ (cmpt_exp_tbl_entries B_cmpt) = [WInt (switcher.encode_entry_point 1 0)]
+
+  (* instantiating C *)
+  ∧ (cmpt_imports C_cmpt) = [switcher_entry]
+  ∧ Forall is_z (cmpt_code C_cmpt) (* only instructions *)
+  ∧ Forall is_z (cmpt_data C_cmpt) (* TODO generalise: either z or in_region *)
+  ∧ (cmpt_exp_tbl_entries C_cmpt) = [WInt (switcher.encode_entry_point 1 0)]
+.
+
+Lemma mk_initial_cmpt_C_disjoint `{Layout: @memory_layout MP} (m : Mem) :
+  is_initial_memory m →
+  mk_initial_switcher switcher_cmpt ∪ mk_initial_assert assert_cmpt ∪ mk_initial_cmpt main_cmpt ∪ mk_initial_cmpt B_cmpt
+    ##ₘ mk_initial_cmpt C_cmpt.
+Proof.
+  intros (Hm & main_imports & main_code & main_data & main_exp_tbl
+          & B_imports & B_code & B_data & B_exp_tbl
+          & C_imports & C_code & C_data & C_exp_tbl
+         ).
+  pose proof cmpts_disjoints as (_ & HmainC & HBC).
+  pose proof switcher_cmpt_disjoints as (_ & _ & HswitcherC).
+  pose proof assert_cmpt_disjoints as (_ & _ & HassertC).
+  do 3 rewrite map_disjoint_union_l.
+  repeat split.
+  - symmetry; apply disjoint_switcher_cmpts_mkinitial; done.
+  - symmetry; apply disjoint_assert_cmpts_mkinitial; done.
+  - apply disjoint_cmpts_mkinitial; done.
+  - apply disjoint_cmpts_mkinitial; done.
+Qed.
+
+Lemma mk_initial_cmpt_B_disjoint `{Layout: @memory_layout MP} (m : Mem) :
+  is_initial_memory m →
+  mk_initial_switcher switcher_cmpt ∪ mk_initial_assert assert_cmpt ∪ mk_initial_cmpt main_cmpt
+    ##ₘ mk_initial_cmpt B_cmpt.
+Proof.
+  intros (Hm & main_imports & main_code & main_data & main_exp_tbl
+          & B_imports & B_code & B_data & B_exp_tbl
+          & C_imports & C_code & C_data & C_exp_tbl
+         ).
+  pose proof cmpts_disjoints as (HmainB & _ & _).
+  pose proof switcher_cmpt_disjoints as (_ & HswitcherB & _).
+  pose proof assert_cmpt_disjoints as (_ & HassertB & _).
+  do 2 rewrite map_disjoint_union_l.
+  repeat split.
+  - symmetry; apply disjoint_switcher_cmpts_mkinitial; done.
+  - symmetry; apply disjoint_assert_cmpts_mkinitial; done.
+  - apply disjoint_cmpts_mkinitial; done.
+Qed.
+
+Lemma mk_initial_cmpt_main_disjoint `{Layout: @memory_layout MP} (m : Mem) :
+  is_initial_memory m →
+  mk_initial_switcher switcher_cmpt ∪ mk_initial_assert assert_cmpt
+    ##ₘ mk_initial_cmpt main_cmpt.
+Proof.
+  intros (Hm & main_imports & main_code & main_data & main_exp_tbl
+          & B_imports & B_code & B_data & B_exp_tbl
+          & C_imports & C_code & C_data & C_exp_tbl
+         ).
+  pose proof switcher_cmpt_disjoints as (HswitcherMain & _ & _).
+  pose proof assert_cmpt_disjoints as (HassertMain & _ & _).
+  rewrite map_disjoint_union_l.
+  repeat split.
+  - symmetry; apply disjoint_switcher_cmpts_mkinitial; done.
+  - symmetry; apply disjoint_assert_cmpts_mkinitial; done.
+Qed.
+
+Section Adequacy.
+  Context (Σ: gFunctors).
+  Context {inv_preg: invGpreS Σ}.
+  Context {mem_preg: gen_heapGpreS Addr Word Σ}.
+  Context {reg_preg: gen_heapGpreS RegName Word Σ}.
+  Context {sreg_preg: gen_heapGpreS SRegName Word Σ}.
+  Context {seal_store_preg: sealStorePreG Σ}.
+  Context {na_invg: na_invG Σ}.
+  Context {sts_preg: STS_preG Addr region_type Σ}.
+  Context {cname : CmptNameG}.
+  Context {heappreg: heapGpreS Σ}.
+  Context `{MP: MachineParameters}.
+  Context {B C : CmptName}.
+  Context { HCNames : CNames = (list_to_set [B;C]) }.
+  Context { HCNamesNoDup : NoDup [B;C] }.
+
+  Notation STS := (leibnizO (STS_states * STS_rels)).
+  Notation STS_STD := (leibnizO (STS_std_states Addr region_type)).
+  Notation CVIEW := (prodO STS_STD STS).
+  Notation WORLD := (gmapO CmptName CVIEW).
+
+  (* TODO move *)
+  Lemma elem_of_dom_std_multiple_update (W : WORLD) (A : CmptName) (a : Addr) (l : list Addr)
+    (ρ: region_type) :
+    is_Some (W !! A) ->
+    a ∈ (dom (std (std_multiple_update W A l ρ) A)) ->
+    a ∈ l \/ a ∈ (dom (std W A)).
+  Proof.
+    intros [WA HWA].
+    induction l as [|a' l] ; intros Ha; first naive_solver.
+    destruct (decide (a = a')) as [|Hna]; simplify_eq; first (left; set_solver).
+    destruct (decide (a ∈ l)) as [|Hnl]; first (left; set_solver).
+    right.
+    rewrite /= HWA /std lookup_insert /std_cview dom_insert_L elem_of_union in Ha.
+    destruct Ha as [Ha|Ha] ; first ( rewrite elem_of_singleton in Ha ; set_solver ).
+    assert (a ∈ dom (std (std_multiple_update W A l ρ) A)).
+    { rewrite /std /std_multiple_update.
+      destruct l; first (rewrite HWA; done).
+      rewrite HWA lookup_insert /std_cview; done.
+    }
+    apply IHl in H. destruct H; done.
+  Qed.
+
+  Definition flagN : namespace := nroot .@ "cmdc" .@ "fail_flag".
+  Definition switcherN : namespace := nroot .@ "cmdc" .@ "switcher_flag".
+  Definition assertN : namespace := nroot .@ "cmdc" .@ "assert_flag".
+
+  Lemma mcdc_adequacy' `{Layout: @memory_layout MP}
+    (reg reg': Reg) (sreg sreg': SReg) (m m': Mem)
+    (es: list cap_lang.expr):
+    is_initial_registers reg →
+    is_initial_sregisters sreg →
+    is_initial_memory m →
+    rtc erased_step ([Seq (Instr Executable)], (reg, sreg, m)) (es, (reg', sreg', m')) →
+    m' !! (flag_assert assert_cmpt) = Some (WInt 0%Z).
+  Proof.
+    intros Hreg Hsreg Hm Hstep.
+    pose proof (@wp_invariance Σ cap_lang _ NotStuck) as WPI. cbn in WPI.
+    pose (fun (c: ExecConf) => c.2 !! (flag_assert assert_cmpt) = Some (WInt 0%Z)) as state_is_good.
+    specialize (WPI (Seq (Instr Executable)) (reg, sreg, m) es (reg', sreg', m')
+                  (state_is_good (reg', sreg', m'))).
+    eapply WPI. 2: assumption. intros Hinv κs. clear WPI.
+
+    pose proof Hm as Hm'.
+    destruct Hm as (Hm
+                    & main_imports & main_code & main_data & main_exp_tbl
+                    & B_imports & B_code & B_data & B_exp_tbl
+                    & C_imports & C_code & C_data & C_exp_tbl
+                   ).
+    iMod (gen_heap_init (reg:Reg)) as (reg_heapg) "(Hreg_ctx & Hreg & _)".
+    iMod (gen_heap_init (sreg:SReg)) as (sreg_heapg) "(Hsreg_ctx & Hsreg & _)".
+    iMod (gen_heap_init (m:Mem)) as (mem_heapg) "(Hmem_ctx & Hmem & _)".
+    iMod (seal_store_init) as (seal_storeg) "Hseal_store".
+
+    unshelve iMod gen_sts_init as (stsg) "Hsts"; eauto. (*XX*)
+    iMod (heap_init) as (heapg) "HRELS".
+    rewrite HCNames.
+    iDestruct (big_sepS_elements with "Hsts") as "Hsts".
+    iDestruct (big_sepS_elements with "HRELS") as "HRELS".
+    setoid_rewrite elements_list_to_set; auto.
+
+    iDestruct (big_sepL_cons with "Hsts") as "[Hsts_B Hsts_C]".
+    iDestruct (big_sepL_cons with "Hsts_C") as "[Hsts_C _]".
+    iDestruct (big_sepL_cons with "HRELS") as "[HRELS_B HRELS_C]".
+    iDestruct (big_sepL_cons with "HRELS_C") as "[HRELS_C _]".
+
+    iMod (@na_alloc Σ na_invg) as (logrel_nais) "Hna".
+
+    pose ceriseg := CeriseG Σ Hinv mem_heapg reg_heapg sreg_heapg.
+    pose logrel_na_invs := Build_logrel_na_invs _ na_invg logrel_nais.
+    pose proof (
+        @cmdc_spec_full Σ ceriseg seal_storeg _ _ _ logrel_na_invs MP B C
+      ) as Spec.
+
+    (* Get initial sregister mtdc *)
+    iDestruct (big_sepM_lookup with "Hsreg") as "Hmtdc"; eauto.
+
+    (* Separate all compartments *)
+    rewrite {2}Hm.
+    rewrite /mk_initial_memory.
+    iDestruct (big_sepM_union with "Hmem") as "[Hmem Hcmpt_C]".
+    { eapply mk_initial_cmpt_C_disjoint; eauto. }
+    iDestruct (big_sepM_union with "Hmem") as "[Hmem Hcmpt_B]".
+    { eapply mk_initial_cmpt_B_disjoint; eauto. }
+    iDestruct (big_sepM_union with "Hmem") as "[Hmem Hcmpt_main]".
+    { eapply mk_initial_cmpt_main_disjoint; eauto. }
+    iDestruct (big_sepM_union with "Hmem") as "[Hcmpt_switcher Hcmpt_assert]".
+    { pose proof assert_switcher_disjoints; symmetry; eapply disjoint_assert_switcher_mkinitial ; eauto. }
+
+    (* Assert *)
+    rewrite /mk_initial_assert.
+    iDestruct (big_sepM_union with "Hcmpt_assert") as "[Hassert Hassert_flag]".
+    { eapply cmpt_assert_flag_mregion_disjoint ; eauto. }
+    iDestruct (big_sepM_union with "Hassert") as "[Hassert Hassert_cap]".
+    { eapply cmpt_assert_cap_mregion_disjoint ; eauto. }
+    rewrite /cmpt_assert_flag_mregion.
+    rewrite /mkregion.
+    rewrite finz_seq_between_singleton.
+    2: { pose proof (assert_flag_size assert_cmpt) as H; solve_addr+H. }
+    cbn.
+    iDestruct (big_sepM_insert with "Hassert_flag") as "[Hassert_flag _]"; first done.
+    iMod (inv_alloc flagN ⊤ (flag_assert assert_cmpt ↦ₐ WInt 0%Z) with "Hassert_flag")%I
+     as "#Hinv_assert_flag".
+    rewrite /cmpt_assert_cap_mregion.
+    rewrite /mkregion.
+    rewrite finz_seq_between_singleton.
+    2: { pose proof (assert_cap_size assert_cmpt) as H; solve_addr+H. }
+    cbn.
+    iDestruct (big_sepM_insert with "Hassert_cap") as "[Hassert_cap _]"; first done.
+
+    rewrite /cmpt_assert_code_mregion.
+    iDestruct (mkregion_prepare with "[Hassert]") as ">Hassert"; auto.
+    { apply (assert_code_size assert_cmpt). }
+    iAssert (assert.assert_inv
+               (b_assert assert_cmpt)
+               (e_assert assert_cmpt)
+               (flag_assert assert_cmpt))
+            with "[Hassert Hassert_cap]" as "Hassert".
+    { rewrite /assert.assert_inv. iExists (cap_assert assert_cmpt).
+      rewrite /codefrag /region_pointsto.
+      replace (b_assert assert_cmpt ^+ length assert_subroutine_instrs)%a
+        with (cap_assert assert_cmpt).
+      2: { pose proof (assert_code_size assert_cmpt); solve_addr+H. }
+      iFrame.
+      iSplit; first (iPureIntro ; apply (assert_code_size assert_cmpt)).
+      iSplit; iPureIntro.
+      + apply (assert_cap_size assert_cmpt).
+      + by rewrite (assert_flag_size assert_cmpt).
+    }
+    iMod (na_inv_alloc logrel.logrel_nais _ assertN _ with "Hassert") as "#Hassert".
+
+    (* Switcher *)
+    rewrite /mk_initial_switcher.
+    iDestruct (big_sepM_union with "Hcmpt_switcher") as "[Hswitcher Hstack]".
+    { eapply cmpt_switcher_stack_mregion_disjoint ; eauto. }
+    iDestruct (big_sepM_union with "Hswitcher") as "[Hswitcher Htrusted_stack]".
+    { eapply cmpt_switcher_trusted_stack_mregion_disjoint ; eauto. }
+
+    rewrite /cmpt_switcher_code_mregion.
+    iDestruct (big_sepM_union with "Hswitcher") as "[Hswitcher_sealing Hswitcher]".
+    { eapply cmpt_switcher_code_stack_mregion_disjoint ; eauto. }
+    iEval (rewrite /mkregion) in "Hswitcher_sealing".
+    rewrite finz_seq_between_singleton.
+    2: { apply (switcher_cc_entry_point switcher_cmpt). }
+    iEval (cbn) in "Hswitcher_sealing".
+    iDestruct (big_sepM_insert with "Hswitcher_sealing") as "[Hswitcher_sealing _]"; first done.
+    iDestruct (mkregion_prepare with "[Hswitcher]") as ">Hswitcher"; auto.
+    { apply (switcher_size switcher_cmpt). }
+    rewrite /cmpt_switcher_trusted_stack_mregion.
+    iDestruct (mkregion_prepare with "[Htrusted_stack]") as ">Htrusted_stack"; auto.
+    { apply (trusted_stack_size switcher_cmpt). }
+    iAssert (switcher_spec.switcher_inv
+               (b_switcher switcher_cmpt)
+               (e_switcher switcher_cmpt)
+               (a_switcher_cc switcher_cmpt)
+               (ot_switcher switcher_cmpt))
+      with "[Hswitcher Hswitcher_sealing Htrusted_stack Hmtdc]" as "Hswitcher".
+    {
+      rewrite /switcher_spec.switcher_inv /codefrag /region_pointsto.
+      replace (a_switcher_cc switcher_cmpt ^+ length switcher_instrs)%a
+        with (e_switcher switcher_cmpt).
+      2: { pose proof (switcher_size switcher_cmpt) as H ; solve_addr+H. }
+      iFrame.
+      iPureIntro.
+      rewrite /SubBounds.
+      clear.
+      pose proof (switcher_size switcher_cmpt).
+      pose proof (switcher_cc_entry_point switcher_cmpt).
+      solve_addr.
+    }
+    iMod (na_inv_alloc logrel.logrel_nais _ switcherN _ with "Hswitcher") as "#Hswitcher".
+
+    (* CMPT B *)
+    assert (
+       (finz.seq_between (cmpt_a_code B_cmpt) (cmpt_e_pcc B_cmpt))  = [cmpt_a_code B_cmpt]
+      ) as Himport_B_size.
+    { admit. }
+
+    iEval (rewrite /mk_initial_cmpt) in "Hcmpt_B".
+    iDestruct (big_sepM_union with "Hcmpt_B") as "[HB HB_etbl]".
+    { eapply cmpt_exp_tbl_disjoint ; eauto. }
+    iDestruct (big_sepM_union with "HB") as "[HB_code HB_data]".
+    { eapply cmpt_cgp_disjoint ; eauto. }
+    rewrite /cmpt_pcc_mregion.
+    iDestruct (big_sepM_union with "HB_code") as "[HB_imports HB_code]".
+    { eapply cmpt_code_disjoint ; eauto. }
+    rewrite B_imports.
+    iEval (rewrite /mkregion) in "HB_imports".
+    rewrite finz_seq_between_singleton.
+    2: { admit. }
+    cbn.
+    iDestruct (big_sepM_insert with "HB_imports") as "[HB_imports _]"; first done.
+    rewrite /cmpt_cgp_mregion.
+    iDestruct (mkregion_prepare with "[HB_code]") as ">HB_code"; auto.
+    { apply (cmpt_code_size B_cmpt). }
+    iDestruct (mkregion_prepare with "[HB_data]") as ">HB_data"; auto.
+    { apply (cmpt_data_size B_cmpt). }
+
+    (* Initialises the world for B *)
+    iAssert (region {[B := (∅, (∅, ∅))]} B) with "[HRELS_B]" as "Hr_B".
+    { rewrite region_eq /region_def. iExists ∅, ∅. iFrame.
+      rewrite /= !dom_empty_L //. repeat iSplit; eauto.
+      - by rewrite /std /std_cview lookup_insert.
+      - rewrite /region_map_def. by rewrite big_sepM_empty. }
+    iMod (extend_region_perm_sepL2 _ {[B := (∅, (∅, ∅))]} B
+            (finz.seq_between (cmpt_a_code B_cmpt) (cmpt_e_pcc B_cmpt))
+            (cmpt_code B_cmpt)
+            RX interpC
+           with "Hsts_B Hr_B [HB_code]") as "(Hr_B & HB_code & Hsts_B)".
+    { done. }
+    { apply Forall_true. intros.
+      by rewrite /std /std_cview lookup_singleton /= lookup_empty.
+    }
+    {
+      iApply (big_sepL2_mono ((fun (_ : nat) (k : finz.finz MemNum) (v : Word) =>
+                                 pointsto k (DfracOwn (pos_to_Qp 1)) v)) with "[HB_code]").
+      - intros k v1 v2 Hv1 Hv2. cbn. iIntros; iFrame.
+        pose proof (Forall_lookup_1 _ _ _ _ B_code Hv2) as Hncap.
+        destruct v2; [| by inversion Hncap..].
+        rewrite fixpoint_interp1_eq /=.
+        iSplit; eauto.
+        iApply interp_weakening.future_priv_mono_interp_z.
+      - iFrame.
+    }
+
+    iMod (extend_region_perm_sepL2 _ _ B
+            (finz.seq_between (cmpt_b_cgp B_cmpt) (cmpt_e_cgp B_cmpt))
+            (cmpt_data B_cmpt)
+            RW interpC
+           with "Hsts_B Hr_B [HB_data]") as "(Hr_B & HB_data & Hsts_B)".
+    { done. }
+    { admit. }
+    {
+      iApply (big_sepL2_mono ((fun (_ : nat) (k : finz.finz MemNum) (v : Word) =>
+                                 pointsto k (DfracOwn (pos_to_Qp 1)) v)) with "[HB_data]").
+      - intros k v1 v2 Hv1 Hv2. cbn. iIntros; iFrame.
+        pose proof (Forall_lookup_1 _ _ _ _ B_data Hv2) as Hncap.
+        destruct v2; [| by inversion Hncap..].
+        rewrite fixpoint_interp1_eq /=.
+        iSplit; eauto.
+        iApply interp_weakening.future_priv_mono_interp_z.
+      - iFrame.
+    }
+
+    iMod (extend_region_perm_sepL2 _ _ B
+            [cmpt_b_pcc B_cmpt]
+            (cmpt_imports B_cmpt)
+            RX interpC
+           with "Hsts_B Hr_B [HB_imports]") as "(Hr_B & HB_imports & Hsts_B)".
+    { done. }
+    { admit. }
+    {
+      iDestruct (switcher_interp with "[$Hswitcher]") as "#Hswitcher_interp".
+      iDestruct (future_priv_mono_interp_switcher with "[$Hswitcher]") as "#Hswitcher_mono".
+      rewrite B_imports /=.
+      iFrame "#∗".
+    }
+    match goal with
+    | H: _ |- context [  (sts_full_world ?W B) ] => set (Winit_B := W)
+    end.
+    set (B_f := (SCap RO Global (cmpt_exp_tbl_pcc B_cmpt) (cmpt_exp_tbl_entries_end B_cmpt) (cmpt_exp_tbl_entries_start B_cmpt))).
+    iAssert ( interp Winit_B B (WSealed (ot_switcher switcher_cmpt) B_f)) with
+      "[HB_etbl HB_code Hr_B HB_data Hsts_B]" as "#Hinterp_B".
+    { admit. } (* TODO we need to define what it means to be safe to share for entry point*)
+    iClear "HB_etbl HB_code HB_data".
+
+    (* CMPT C *)
+    assert (
+       (finz.seq_between (cmpt_a_code C_cmpt) (cmpt_e_pcc C_cmpt)) = [cmpt_a_code C_cmpt]
+      ) as Himport_C_size.
+    { admit. }
+    iEval (rewrite /mk_initial_cmpt) in "Hcmpt_C".
+    iDestruct (big_sepM_union with "Hcmpt_C") as "[HC HC_etbl]".
+    { eapply cmpt_exp_tbl_disjoint ; eauto. }
+    iDestruct (big_sepM_union with "HC") as "[HC_code HC_data]".
+    { eapply cmpt_cgp_disjoint ; eauto. }
+    rewrite /cmpt_pcc_mregion.
+    iDestruct (big_sepM_union with "HC_code") as "[HC_imports HC_code]".
+    { eapply cmpt_code_disjoint ; eauto. }
+    rewrite C_imports.
+    iEval (rewrite /mkregion) in "HC_imports".
+    rewrite finz_seq_between_singleton.
+    2: { admit. }
+    iDestruct (big_sepM_insert with "HC_imports") as "[HC_imports _]"; first done.
+    rewrite /cmpt_cgp_mregion.
+    iDestruct (mkregion_prepare with "[HC_code]") as ">HC_code"; auto.
+    { apply (cmpt_code_size C_cmpt). }
+    iDestruct (mkregion_prepare with "[HC_data]") as ">HC_data"; auto.
+    { apply (cmpt_data_size C_cmpt). }
+
+    (* Initialises the world for C *)
+    iAssert (region {[C := (∅, (∅, ∅))]} C) with "[HRELS_C]" as "Hr_C".
+    { rewrite region_eq /region_def. iExists ∅, ∅. iFrame.
+      rewrite /= !dom_empty_L //. repeat iSplit; eauto.
+      - by rewrite /std /std_cview lookup_insert.
+      - rewrite /region_map_def. by rewrite big_sepM_empty. }
+
+    iMod (extend_region_perm_sepL2 _ {[C := (∅, (∅, ∅))]} C
+            (finz.seq_between (cmpt_a_code C_cmpt) (cmpt_e_pcc C_cmpt))
+            (cmpt_code C_cmpt)
+            RX interpC
+           with "Hsts_C Hr_C [HC_code]") as "(Hr_C & HC_code & Hsts_C)".
+    { done. }
+    { apply Forall_true. intros.
+      by rewrite /std /std_cview lookup_singleton /= lookup_empty.
+    }
+    {
+      iApply (big_sepL2_mono ((fun (_ : nat) (k : finz.finz MemNum) (v : Word) =>
+                                 pointsto k (DfracOwn (pos_to_Qp 1)) v)) with "[HC_code]").
+      - intros k v1 v2 Hv1 Hv2. cbn. iIntros; iFrame.
+        pose proof (Forall_lookup_1 _ _ _ _ C_code Hv2) as Hncap.
+        destruct v2; [| by inversion Hncap..].
+        rewrite fixpoint_interp1_eq /=.
+        iSplit; eauto.
+        iApply interp_weakening.future_priv_mono_interp_z.
+      - iFrame.
+    }
+    iMod (extend_region_perm_sepL2 _ _ C
+            (finz.seq_between (cmpt_b_cgp C_cmpt) (cmpt_e_cgp C_cmpt))
+            (cmpt_data C_cmpt)
+            RW interpC
+           with "Hsts_C Hr_C [HC_data]") as "(Hr_C & HC_data & Hsts_C)".
+    { done. }
+    { admit. }
+    {
+      iApply (big_sepL2_mono ((fun (_ : nat) (k : finz.finz MemNum) (v : Word) =>
+                                 pointsto k (DfracOwn (pos_to_Qp 1)) v)) with "[HC_data]").
+      - intros k v1 v2 Hv1 Hv2. cbn. iIntros; iFrame.
+        pose proof (Forall_lookup_1 _ _ _ _ C_data Hv2) as Hncap.
+        destruct v2; [| by inversion Hncap..].
+        rewrite fixpoint_interp1_eq /=.
+        iSplit; eauto.
+        iApply interp_weakening.future_priv_mono_interp_z.
+      - iFrame.
+    }
+
+    iMod (extend_region_perm_sepL2 _ _ C
+            [cmpt_b_pcc C_cmpt]
+            (cmpt_imports C_cmpt)
+            RX interpC
+           with "Hsts_C Hr_C [HC_imports]") as "(Hr_C & HC_imports & Hsts_C)".
+    { done. }
+    { admit. }
+    {
+      iDestruct (switcher_interp with "[$Hswitcher]") as "#Hswitcher_interp".
+      iDestruct (future_priv_mono_interp_switcher with "[$Hswitcher]") as "#Hswitcher_mono".
+      rewrite C_imports /=.
+      iFrame "#∗".
+    }
+    match goal with
+    | H: _ |- context [  (sts_full_world ?W C) ] => set (Winit_C := W)
+    end.
+    set (C_g := (SCap RO Global (cmpt_exp_tbl_pcc C_cmpt) (cmpt_exp_tbl_entries_end C_cmpt)
+                   (cmpt_exp_tbl_entries_start C_cmpt))).
+    iAssert ( interp Winit_C C (WSealed (ot_switcher switcher_cmpt) C_g)) with
+      "[HC_etbl HC_code Hr_C HC_data Hsts_C]" as "#Hinterp_C".
+    { admit. } (* TODO we need to define what it means to be safe to share for entry point*)
+    iClear "HC_etbl HC_code HC_data".
+
+    (* CMPT MAIN *)
+    iEval (rewrite /mk_initial_cmpt) in "Hcmpt_main".
+    iDestruct (big_sepM_union with "Hcmpt_main") as "[Hmain Hmain_etbl]".
+    { eapply cmpt_exp_tbl_disjoint ; eauto. }
+    iDestruct (big_sepM_union with "Hmain") as "[Hmain_code Hmain_data]".
+    { eapply cmpt_cgp_disjoint ; eauto. }
+    rewrite /cmpt_pcc_mregion.
+    iDestruct (big_sepM_union with "Hmain_code") as "[Hmain_imports Hmain_code]".
+    { admit. }
+    rewrite /cmpt_cgp_mregion.
+    iDestruct (mkregion_prepare with "[Hmain_imports]") as ">Hmain_imports"; auto.
+    { apply (cmpt_import_size main_cmpt). }
+    iDestruct (mkregion_prepare with "[Hmain_code]") as ">Hmain_code"; auto.
+    { apply (cmpt_code_size main_cmpt). }
+    iDestruct (mkregion_prepare with "[Hmain_data]") as ">Hmain_data"; auto.
+    { apply (cmpt_data_size main_cmpt). }
+    iAssert (
+       [[(cmpt_b_pcc main_cmpt),(cmpt_a_code main_cmpt)]]↦ₐ[[cmpt_imports main_cmpt]]
+     )%I with "[Hmain_imports]" as "Hmain_imports"; first done.
+    iAssert (
+       [[(cmpt_b_cgp main_cmpt),(cmpt_e_cgp main_cmpt)]]↦ₐ[[cmpt_data main_cmpt]]
+     )%I with "[Hmain_data]" as "Hmain_data"; first done.
+    iAssert (
+      codefrag (cmpt_a_code main_cmpt) (cmpt_code main_cmpt)
+     )%I with "[Hmain_code]" as "Hmain_code".
+    { rewrite /codefrag.
+      replace (cmpt_a_code main_cmpt ^+ length (cmpt_code main_cmpt))%a
+        with (cmpt_e_pcc main_cmpt).
+      2: { pose proof (cmpt_code_size main_cmpt) as H ; solve_addr+H. }
+      done.
+    }
+    rewrite main_imports main_code main_data.
+
+    (* Compartment's stack *)
+    rewrite /cmpt_switcher_stack_mregion.
+    iDestruct (mkregion_prepare with "[Hstack]") as ">Hstack"; auto.
+    { apply (stack_size switcher_cmpt). }
+    iAssert (
+        [[(b_stack switcher_cmpt), (e_stack switcher_cmpt)]]↦ₐ[[(stack_content switcher_cmpt)]]
+      )%I with "[Hstack]" as "Hstack"; first done.
+
+    (* Extract registers *)
+    destruct Hreg as (HPC & Hcgp & Hcsp & Hreg).
+    iDestruct (big_sepM_delete _ _ PC with "Hreg") as "[HPC Hreg]"; first by simplify_map_eq.
+    iDestruct (big_sepM_delete _ _ cgp with "Hreg") as "[Hcgp Hreg]"; first by simplify_map_eq.
+    iDestruct (big_sepM_delete _ _ csp with "Hreg") as "[Hcsp Hreg]"; first by simplify_map_eq.
+
+    iPoseProof (Spec _ _ _ _ _ _ _ _ _ _ _ _ _ _ _
+                  _ _ _ _ _ (fun _ => True)%I assertN switcherN
+                 with "[ $Hassert $Hswitcher $Hna
+                        $Hr_B $Hr_C $Hsts_B $Hsts_C
+                        $HPC $Hcgp $Hcsp $Hreg
+                        $Hmain_imports $Hmain_code $Hmain_data $Hstack
+                        $Hinterp_B $Hinterp_C
+                        ]") as "Hspec"; eauto.
+    { rewrite !dom_delete_L.
+      rewrite regmap_full_dom; first done.
+      intros r.
+      destruct (decide (r = PC)); simplify_eq.
+      { eexists; eapply HPC. }
+      destruct (decide (r = cgp)); simplify_eq.
+      { eexists; eapply Hcgp. }
+      destruct (decide (r = csp)); simplify_eq.
+      { eexists; eapply Hcsp. }
+      eexists (WInt 0).
+      apply Hreg.
+      clear -n n0 n1; set_solver.
+    }
+   { intros r Hdom.
+     rewrite !dom_delete_L in Hdom.
+     destruct (decide (r = PC)); simplify_eq.
+     { set_solver+Hdom. }
+     destruct (decide (r = cgp)); simplify_eq.
+     { set_solver+Hdom. }
+     destruct (decide (r = csp)); simplify_eq.
+     { set_solver+Hdom. }
+     rewrite !lookup_delete_ne //.
+     apply Hreg.
+     clear -n n0 n1; set_solver.
+    }
+    { rewrite /SubBounds.
+      pose proof (cmpt_import_size main_cmpt) as Hmain_imports.
+      pose proof (cmpt_code_size main_cmpt) as Hmain_code.
+      rewrite -main_code.
+      solve_addr+Hmain_imports Hmain_code.
+    }
+    { pose proof (cmpt_data_size main_cmpt) as Hmain_data.
+      by rewrite -main_data.
+    }
+    { pose proof (cmpt_import_size main_cmpt) as Hmain_imports.
+      by rewrite -Hmain_imports main_imports.
+    }
+    { subst Winit_B.
+      intro Hcontra.
+      apply elem_of_dom_std_multiple_update in Hcontra.
+      2:{
+        rewrite /std_multiple_update.
+        destruct (finz.seq_between (cmpt_a_code B_cmpt) (cmpt_e_pcc B_cmpt)),
+                   (finz.seq_between (cmpt_b_cgp B_cmpt) (cmpt_e_cgp B_cmpt))
+                   ; rewrite lookup_singleton ; try done
+                   ; rewrite !lookup_insert ; try done.
+      }
+      destruct Hcontra as [Hcontra|Hcontra].
+      - admit.
+      - apply elem_of_dom_std_multiple_update in Hcontra.
+        2: {
+          rewrite /std_multiple_update.
+          destruct (finz.seq_between (cmpt_a_code B_cmpt) (cmpt_e_pcc B_cmpt))
+            ; rewrite !lookup_singleton ; try done
+            ; rewrite !lookup_insert ; try done.
+        }
+        destruct Hcontra as [Hcontra|Hcontra].
+        + admit.
+        + apply elem_of_dom_std_multiple_update in Hcontra; last by rewrite lookup_singleton.
+          destruct Hcontra as [Hcontra|Hcontra].
+          * admit.
+          * rewrite /std lookup_insert /std_cview /= dom_empty_L in Hcontra; set_solver+Hcontra.
+    }
+    { subst Winit_C.
+      intro Hcontra.
+      apply elem_of_dom_std_multiple_update in Hcontra.
+      2:{
+        rewrite /std_multiple_update.
+        destruct (finz.seq_between (cmpt_a_code C_cmpt) (cmpt_e_pcc C_cmpt)),
+                   (finz.seq_between (cmpt_b_cgp C_cmpt) (cmpt_e_cgp C_cmpt))
+                   ; rewrite lookup_singleton ; try done
+                   ; rewrite !lookup_insert ; try done.
+      }
+      destruct Hcontra as [Hcontra|Hcontra].
+      - admit.
+      - apply elem_of_dom_std_multiple_update in Hcontra.
+        2: {
+          rewrite /std_multiple_update.
+          destruct (finz.seq_between (cmpt_a_code C_cmpt) (cmpt_e_pcc C_cmpt))
+            ; rewrite !lookup_singleton ; try done
+            ; rewrite !lookup_insert ; try done.
+        }
+        destruct Hcontra as [Hcontra|Hcontra].
+        + admit.
+        + apply elem_of_dom_std_multiple_update in Hcontra; last by rewrite lookup_singleton.
+          destruct Hcontra as [Hcontra|Hcontra].
+          * admit.
+          * rewrite /std lookup_insert /std_cview /= dom_empty_L in Hcontra; set_solver+Hcontra.
+    }
+    { clear.
+      pose proof (stack_size switcher_cmpt) as Hstacksize.
+      replace (e_stack switcher_cmpt) with ( (b_stack switcher_cmpt) ^+ length
+                                               (stack_content switcher_cmpt))%a
+      by (by apply finz_incr_eq).
+      rewrite /finz.dist; solve_addr.
+    }
+    { iNext; iIntros "H". proofmode.wp_end; by iLeft. }
+
+    iModIntro.
+    iExists (fun σ _ _ => ( ((gen_heap_interp σ.1.1) ∗ (gen_heap_interp σ.1.2)) ∗ (gen_heap_interp σ.2)))%I.
+    iExists (fun _ => True)%I. cbn. iFrame.
+
+    iIntros "[ [Hreg' Hsreg'] Hmem']". iExists (⊤ ∖ ↑flagN).
+    iInv flagN as ">Hflag" "Hclose".
+    iDestruct (gen_heap_valid with "Hmem' Hflag") as %Hm'_flag.
+    iModIntro. iPureIntro. rewrite /state_is_good //=.
+  Admitted.
+End Adequacy.
