theories/examples/cmdc/cmdc_spec.v
@@ -1,0 +1,796 @@
+From iris.proofmode Require Import proofmode.
+From cap_machine Require Import region_invariants_allocation interp_weakening.
+From cap_machine Require Import logrel rules proofmode.
+From cap_machine Require Import fetch assert switcher_spec cmdc.
+
+Section CMDC.
+  Context
+    {Σ:gFunctors}
+    {ceriseg:ceriseG Σ} {sealsg: sealStoreG Σ}
+    {Cname : CmptNameG}
+    {stsg : STSG Addr region_type Σ} {heapg : heapGS Σ}
+    {nainv: logrel_na_invs Σ}
+    `{MP: MachineParameters}.
+  Context {B C : CmptName}.
+
+  Notation STS := (leibnizO (STS_states * STS_rels)).
+  Notation STS_STD := (leibnizO (STS_std_states Addr region_type)).
+  Notation CVIEW := (prodO STS_STD STS).
+  Notation WORLD := (gmapO CmptName CVIEW).
+
+  Ltac iHide0 irisH coqH :=
+    let coqH := fresh coqH in
+    match goal with
+    | h: _ |- context [ environments.Esnoc _ (INamed irisH) ?prop ] =>
+        set (coqH := prop)
+    end.
+
+  Tactic Notation "iHide" constr(irisH) "as" ident(coqH) :=
+    iHide0 irisH coqH.
+
+  Lemma cmdc_spec
+
+    (pc_b pc_e pc_a : Addr)
+    (cgp_b cgp_e : Addr)
+    (csp_b csp_e : Addr)
+    (rmap : Reg)
+
+    (b_switcher e_switcher a_cc_switcher : Addr) (ot_switcher : OType)
+    (b_assert e_assert : Addr) (a_flag : Addr)
+    (B_f C_g : Sealable)
+
+    (W_init_B : WORLD)
+    (W_init_C : WORLD)
+
+    (csp_content : list Word)
+
+    (φ : language.val cap_lang -> iProp Σ)
+    (Nassert Nswitcher : namespace)
+    (E : coPset)
+    :
+
+    let imports :=
+     cmdc_main_imports b_switcher e_switcher a_cc_switcher ot_switcher b_assert e_assert B_f C_g
+    in
+
+    ↑Nswitcher ⊆ E ->
+    ↑Nassert ⊆ E ->
+
+    dom rmap = all_registers_s ∖ {[ PC ; cgp ; csp]} ->
+    (forall r, r ∈ dom rmap -> rmap !! r = Some (WInt 0) ) ->
+    SubBounds pc_b pc_e pc_a (pc_a ^+ length cmdc_main_code)%a ->
+
+    (cgp_b + length cmdc_main_data)%a = Some cgp_e ->
+    (pc_b + length imports)%a = Some pc_a ->
+
+    cgp_b ∉ dom (std W_init_B B) ->
+    (cgp_b ^+ 1)%a ∉ dom (std W_init_C C) ->
+
+    length csp_content = finz.dist csp_b csp_e ->
+
+    (
+      na_inv logrel_nais Nassert (assert_inv b_assert e_assert a_flag)
+      ∗ na_inv logrel_nais Nswitcher (switcher_inv b_switcher e_switcher a_cc_switcher ot_switcher)
+      ∗ na_own logrel_nais E
+
+      (* initial register file *)
+      ∗ PC ↦ᵣ WCap RX Global pc_b pc_e pc_a
+      ∗ cgp ↦ᵣ WCap RW Global cgp_b cgp_e cgp_b
+      ∗ csp ↦ᵣ WCap RWL Local csp_b csp_e csp_b
+      ∗ ( [∗ map] r↦w ∈ rmap, r ↦ᵣ w )
+
+      (* initial memory layout *)
+      ∗ [[ pc_b , pc_a ]] ↦ₐ [[ imports ]]
+      ∗ codefrag pc_a cmdc_main_code
+      ∗ [[ cgp_b , cgp_e ]] ↦ₐ [[ cmdc_main_data ]]
+      ∗ [[ csp_b , csp_e ]] ↦ₐ [[ csp_content ]]
+
+      ∗ region W_init_B B ∗ sts_full_world W_init_B B
+      ∗ region W_init_C C ∗ sts_full_world W_init_C C
+
+      ∗ interp W_init_B B (WSealed ot_switcher B_f)
+      ∗ interp W_init_C C (WSealed ot_switcher C_g)
+
+      ∗ ▷ (
+            na_own logrel_nais E
+              -∗ WP Instr Halted {{ λ v, φ v ∨ ⌜v = FailedV⌝ }})
+      ⊢ WP Seq (Instr Executable) {{ λ v, φ v ∨ ⌜v = FailedV⌝ }})%I.
+  Proof.
+    intros imports; subst imports.
+    iIntros (HNswitcherE HNassertE Hrmap_dom Hrmap_init HsubBounds
+               Hcgp_contiguous Himports_contiguous Hcgp_b Hcgp_c Hlen_stack)
+      "(#Hassert & #Hswitcher & Hna
+      & HPC & Hcgp & Hcsp & Hrmap
+      & Himports_main & Hcode_main & Hcgp_main & Hcsp_stk
+      & HWreg_B & HWstd_full_B
+      & HWreg_C & HWstd_full_C
+      & #Hinterp_Winit_B_f & #Hinterp_Winit_C_g
+      & Hφ)".
+    codefrag_facts "Hcode_main"; rename H into Hpc_contiguous ; clear H0.
+
+    (* TODO tactic for extracting register.... *)
+    (* --- Extract registers ca0 ctp ct0 ct1 cs0 cs1 cra --- *)
+    assert ( rmap !! ca0 = Some (WInt 0) ) as Hwca0.
+    { apply Hrmap_init. rewrite Hrmap_dom.
+      apply elem_of_difference; split; [apply all_registers_s_correct|set_solver].
+    }
+    iDestruct (big_sepM_delete _ _ ca0 with "Hrmap") as "[Hca0 Hrmap]"; first by simplify_map_eq.
+    assert ( rmap !! ctp = Some (WInt 0) ) as Hwctp.
+    { apply Hrmap_init. rewrite Hrmap_dom.
+      apply elem_of_difference; split; [apply all_registers_s_correct|set_solver].
+    }
+    iDestruct (big_sepM_delete _ _ ctp with "Hrmap") as "[Hctp Hrmap]"; first by simplify_map_eq.
+    assert ( rmap !! ct0 = Some (WInt 0) ) as Hwct0.
+    { apply Hrmap_init. rewrite Hrmap_dom.
+      apply elem_of_difference; split; [apply all_registers_s_correct|set_solver].
+    }
+    iDestruct (big_sepM_delete _ _ ct0 with "Hrmap") as "[Hct0 Hrmap]"; first by simplify_map_eq.
+    assert ( rmap !! ct1 = Some (WInt 0) ) as Hwct1.
+    { apply Hrmap_init. rewrite Hrmap_dom.
+      apply elem_of_difference; split; [apply all_registers_s_correct|set_solver].
+    }
+    iDestruct (big_sepM_delete _ _ ct1 with "Hrmap") as "[Hct1 Hrmap]"; first by simplify_map_eq.
+    assert ( rmap !! cs0 = Some (WInt 0) ) as Hwcs0.
+    { apply Hrmap_init. rewrite Hrmap_dom.
+      apply elem_of_difference; split; [apply all_registers_s_correct|set_solver].
+    }
+    iDestruct (big_sepM_delete _ _ cs0 with "Hrmap") as "[Hcs0 Hrmap]"; first by simplify_map_eq.
+    assert ( rmap !! cs1 = Some (WInt 0) ) as Hwcs1.
+    { apply Hrmap_init. rewrite Hrmap_dom.
+      apply elem_of_difference; split; [apply all_registers_s_correct|set_solver].
+    }
+    iDestruct (big_sepM_delete _ _ cs1 with "Hrmap") as "[Hcs1 Hrmap]"; first by simplify_map_eq.
+    assert ( rmap !! cra = Some (WInt 0) ) as Hwcra.
+    { apply Hrmap_init. rewrite Hrmap_dom.
+      apply elem_of_difference; split; [apply all_registers_s_correct|set_solver].
+    }
+    iDestruct (big_sepM_delete _ _ cra with "Hrmap") as "[Hcra Hrmap]"; first by simplify_map_eq.
+
+    (* Extract the addresses of b and c *)
+    iDestruct (region_pointsto_cons with "Hcgp_main") as "[Hcgp_b Hcgp_main]".
+    { transitivity (Some (cgp_b ^+ 1)%a); auto; solve_addr. }
+    { solve_addr. }
+    iDestruct (region_pointsto_cons with "Hcgp_main") as "[Hcgp_c _]".
+    { transitivity (Some (cgp_b ^+ 2)%a); auto; solve_addr. }
+    { solve_addr. }
+
+    (* Extract the imports *)
+    iDestruct (region_pointsto_cons with "Himports_main") as "[Himport_switcher Himports_main]".
+    { transitivity (Some (pc_b ^+ 1)%a); auto; solve_addr. }
+    { solve_addr. }
+    iDestruct (region_pointsto_cons with "Himports_main") as "[Himport_assert Himports_main]".
+    { transitivity (Some (pc_b ^+ 2)%a); auto; solve_addr. }
+    { solve_addr. }
+    iDestruct (region_pointsto_cons with "Himports_main") as "[Himport_B_f Himports_main]".
+    { transitivity (Some (pc_b ^+ 3)%a); auto; solve_addr. }
+    { solve_addr. }
+    iDestruct (region_pointsto_cons with "Himports_main") as "[Himport_C_g _]".
+    { transitivity (Some (pc_b ^+ 4)%a); auto; solve_addr. }
+    { solve_addr. }
+
+
+    (* --------------------------------------------------- *)
+    (* ----------------- Start the proof ----------------- *)
+    (* --------------------------------------------------- *)
+
+
+
+    (* --------------------------------------------------- *)
+    (* ----------------- BLOCK 0 : INIT ------------------ *)
+    (* --------------------------------------------------- *)
+
+    focus_block_0 "Hcode_main" as "Hcode" "Hcont"; iHide "Hcont" as hcont.
+    (* Store cgp 0%Z; *)
+    iInstr "Hcode".
+    { solve_addr. }
+    iHide "Hφ" as hφ.
+    (* Mov ca0 cgp; *)
+    iInstr "Hcode".
+    (* Lea cgp 1%Z; *)
+    iInstr "Hcode".
+    { transitivity (Some (cgp_b ^+ 1)%a); auto; solve_addr. }
+    (* Store cgp 0%Z; *)
+    iInstr "Hcode".
+    { solve_addr. }
+    (* GetA ct0 ca0; *)
+    iInstr "Hcode".
+    (* Add ct1 ct0 1%Z; *)
+    iInstr "Hcode".
+    (* Subseg ca0 ct0 ct1  *)
+    iInstr "Hcode".
+    { transitivity (Some (cgp_b ^+ 1)%a); auto; solve_addr. }
+    { solve_addr. }
+    subst hcont; unfocus_block "Hcode" "Hcont" as "Hcode_main".
+
+    (* --------------------------------------------------- *)
+    (* -------------- BLOCK 1 and 2 : FETCH -------------- *)
+    (* --------------------------------------------------- *)
+
+    focus_block 1 "Hcode_main" as a_fetch1 Ha_fetch1 "Hcode" "Hcont"; iHide "Hcont" as hcont.
+    iApply (fetch_spec with "[- $HPC $Hctp $Hct0 $Hct1 $Hcode]"); eauto.
+    { solve_addr. }
+    replace (pc_b ^+ 0)%a with pc_b by solve_addr.
+    iFrame "Himport_switcher".
+    iNext ; iIntros "(HPC & Hctp & Hct0 & Hct1 & Hcode & Himport_switcher)".
+    iEval (cbn) in "Hctp".
+    subst hcont; unfocus_block "Hcode" "Hcont" as "Hcode_main".
+
+    focus_block 2 "Hcode_main" as a_fetch2 Ha_fetch2 "Hcode" "Hcont"; iHide "Hcont" as hcont.
+    iApply (fetch_spec with "[- $HPC $Hcs0 $Hct0 $Hct1 $Hcode $Himport_B_f]"); eauto.
+    { solve_addr. }
+    iNext ; iIntros "(HPC & Hcs0 & Hct0 & Hct1 & Hcode & Himport_B_f)".
+    iEval (cbn) in "Hcs0".
+    subst hcont; unfocus_block "Hcode" "Hcont" as "Hcode_main".
+
+
+    (* --------------------------------------------------- *)
+    (* ----------------- BLOCK 3: CALL B ----------------- *)
+    (* --------------------------------------------------- *)
+
+    (* ---- call B ---- *)
+    focus_block 3 "Hcode_main" as a_callB Ha_callB "Hcode" "Hcont"; iHide "Hcont" as hcont.
+    iInstr "Hcode".
+
+    (* -- separate argument registers -- *)
+    assert ( rmap !! ca1 = Some (WInt 0) ) as Hwca1.
+    { apply Hrmap_init. rewrite Hrmap_dom.
+      apply elem_of_difference; split; [apply all_registers_s_correct|set_solver].
+    }
+    iDestruct (big_sepM_delete _ _ ca1 with "Hrmap") as "[Hca1 Hrmap]"; first by simplify_map_eq.
+    assert ( rmap !! ca2 = Some (WInt 0) ) as Hwca2.
+    { apply Hrmap_init. rewrite Hrmap_dom.
+      apply elem_of_difference; split; [apply all_registers_s_correct|set_solver].
+    }
+    iDestruct (big_sepM_delete _ _ ca2 with "Hrmap") as "[Hca2 Hrmap]"; first by simplify_map_eq.
+    assert ( rmap !! ca3 = Some (WInt 0) ) as Hwca3.
+    { apply Hrmap_init. rewrite Hrmap_dom.
+      apply elem_of_difference; split; [apply all_registers_s_correct|set_solver].
+    }
+    iDestruct (big_sepM_delete _ _ ca3 with "Hrmap") as "[Hca3 Hrmap]"; first by simplify_map_eq.
+    assert ( rmap !! ca4 = Some (WInt 0) ) as Hwca4.
+    { apply Hrmap_init. rewrite Hrmap_dom.
+      apply elem_of_difference; split; [apply all_registers_s_correct|set_solver].
+    }
+    iDestruct (big_sepM_delete _ _ ca4 with "Hrmap") as "[Hca4 Hrmap]"; first by simplify_map_eq.
+    assert ( rmap !! ca5 = Some (WInt 0) ) as Hwca5.
+    { apply Hrmap_init. rewrite Hrmap_dom.
+      apply elem_of_difference; split; [apply all_registers_s_correct|set_solver].
+    }
+    iDestruct (big_sepM_delete _ _ ca5 with "Hrmap") as "[Hca5 Hrmap]"; first by simplify_map_eq.
+
+    set ( rmap_arg :=
+           {[ ca0 := WCap RW Global cgp_b (cgp_b ^+ 1)%a cgp_b;
+              ca1 := WInt 0;
+              ca2 := WInt 0;
+              ca3 := WInt 0;
+              ca4 := WInt 0;
+              ca5 := WInt 0;
+              ct0 := WInt 0
+           ]} : Reg
+        ).
+
+    rewrite !(delete_commute _ _ ct1).
+    iDestruct (big_sepM_insert _ _ ct1 with "[$Hrmap $Hct1]") as "Hrmap"; first by simplify_map_eq.
+    rewrite insert_delete_insert.
+    repeat (rewrite -delete_insert_ne //).
+    rewrite !(delete_commute _ _ ctp).
+    iDestruct (big_sepM_insert _ _ ctp with "[$Hrmap $Hctp]") as "Hrmap"; first by simplify_map_eq.
+    rewrite insert_delete_insert.
+    repeat (rewrite -delete_insert_ne //).
+
+    set (rmap' := (delete ca5 _)).
+
+    iMod (extend_region_perm _ _ _ _ _ RW interpC
+        with "[] [$HWstd_full_B] [$HWreg_B] [$Hcgp_b] []")
+      as "(HWreg_B & Hrel_cgp_b & HWstd_full_B)".
+    { done. }
+    { done. }
+    { iApply future_priv_mono_interp_z. }
+    { cbn; iEval (rewrite fixpoint_interp1_eq); done. }
+
+    set (W1 := <s[(B,cgp_b):=Permanent]s>W_init_B).
+    assert (related_sts_priv_world W_init_B W1 B) as HWinit_privB_W1.
+    { subst W1; by eapply related_sts_priv_world_fresh_Permanent. }
+
+    iAssert (interp W1 B (WSealed ot_switcher B_f)) as "#Hinterp_W1_B_f".
+    { iApply monotone.interp_monotone_sd; eauto. }
+
+    iAssert (interp W1 B (WCap RW Global cgp_b (cgp_b ^+ 1)%a cgp_b)) as "#Hinterp_W1_B_b".
+    { iEval (cbn). iEval (rewrite fixpoint_interp1_eq). iEval (cbn).
+      rewrite finz_seq_between_cons; last solve_addr.
+      rewrite finz_seq_between_empty; last solve_addr.
+      iApply big_sepL_singleton.
+      iExists RW, interp.
+      iEval (cbn).
+      iSplit; first done.
+      iSplit; first (iPureIntro ; by apply persistent_cond_interp).
+      iSplit; first iFrame "Hrel_cgp_b".
+      iSplit; first (iNext ; by iApply zcond_interp).
+      iSplit; first (iNext ; by iApply rcond_interp).
+      iSplit; first (iNext ; by iApply wcond_interp).
+      subst W1.
+      iSplit.
+      + iApply monoReq_interp; last done.
+        rewrite /std_update /std_update_cview /std /std_cview.
+        destruct (W_init_B !! B); rewrite !lookup_insert; done.
+      + iPureIntro.
+        rewrite /std_update /std_update_cview /std /std_cview.
+        destruct (W_init_B !! B); rewrite !lookup_insert; done.
+    }
+
+    iAssert ([∗ map] rarg↦warg ∈ rmap_arg, rarg ↦ᵣ warg ∗ interp W1 B warg )%I
+      with "[Hca0 Hca1 Hca2 Hca3 Hca4 Hca5 Hct0]" as "Hrmap_arg".
+    { subst rmap_arg.
+      iAssert (interp W1 B (WInt 0)) as "Hinterp_0".
+      { iEval (rewrite fixpoint_interp1_eq); done. }
+      repeat (iApply big_sepM_insert; [done|iFrame "∗#"]).
+      done.
+    }
+
+    iApply (switcher_cc_specification _ _ W1 W1 with
+             "[- $Hswitcher $Hna
+              $HPC $Hcgp $Hcra $Hcsp $Hcs0 $Hcs1 $Hrmap_arg $Hrmap
+              $Hcsp_stk $HWreg_B $HWstd_full_B
+              $Hinterp_W1_B_f]"); auto.
+    { set_solver. }
+    { subst rmap'.
+      repeat (rewrite dom_delete_L); repeat (rewrite dom_insert_L).
+      rewrite Hrmap_dom; set_solver.
+    }
+    iSplitR.
+    { iIntros "(Hcsp_stk & HWreg_B & Hstd_full_B)". iModIntro; iFrame. }
+    iNext. subst rmap'.
+    iIntros "H".
+    iDestruct "H"
+      as (W2 rmap') "(%HW1_pubB_W2 & %Hdom_rmap'
+                      & Hna & HWreg_B & HWstd_full_B
+                      & HPC & Hcgp & Hcra & Hcsp & Hca0 & Hca1
+                      & Hrmap & Hcsp_stk)".
+    iDestruct "Hca0" as (warg0) "[Hca0 _]".
+    iDestruct "Hca1" as (warg1) "[Hca1 _]".
+    rewrite updatePcPerm_seal_perm_sentry; last solve_pure.
+
+    iDestruct (big_sepM_sep with "Hrmap") as "[Hrmap Hrmap_zero]".
+    iDestruct (big_sepM_pure with "Hrmap_zero") as "%Hrmap_zero".
+    assert (∀ r : RegName, r ∈ dom rmap' → rmap' !! r = Some (WInt 0)) as Hrmap_init'.
+    { intros r Hr.
+      rewrite elem_of_dom in Hr. destruct Hr as [wr Hr].
+      pose proof Hr as Hr'.
+      eapply map_Forall_lookup in Hr'; eauto.
+      by cbn in Hr' ; simplify_eq.
+    }
+    iClear "Hrmap_zero".
+
+    (* ---- extract the needed registers ctp ct0 ct1 ct2 ct3 ct4 cs0 ----  *)
+    assert ( rmap' !! ctp = Some (WInt 0) ) as Hwctp'.
+    { apply Hrmap_init'. rewrite Hdom_rmap'.
+      apply elem_of_difference; split; [apply all_registers_s_correct|set_solver].
+    }
+    iDestruct (big_sepM_delete _ _ ctp with "Hrmap") as "[Hctp Hrmap]"; first by simplify_map_eq.
+    assert ( rmap' !! ct0 = Some (WInt 0) ) as Hwct0'.
+    { apply Hrmap_init'. rewrite Hdom_rmap'.
+      apply elem_of_difference; split; [apply all_registers_s_correct|set_solver].
+    }
+    iDestruct (big_sepM_delete _ _ ct0 with "Hrmap") as "[Hct0 Hrmap]"; first by simplify_map_eq.
+    assert ( rmap' !! ct1 = Some (WInt 0) ) as Hwct1'.
+    { apply Hrmap_init'. rewrite Hdom_rmap'.
+      apply elem_of_difference; split; [apply all_registers_s_correct|set_solver].
+    }
+    iDestruct (big_sepM_delete _ _ ct1 with "Hrmap") as "[Hct1 Hrmap]"; first by simplify_map_eq.
+    assert ( rmap' !! ct2 = Some (WInt 0) ) as Hwct2'.
+    { apply Hrmap_init'. rewrite Hdom_rmap'.
+      apply elem_of_difference; split; [apply all_registers_s_correct|set_solver].
+    }
+    iDestruct (big_sepM_delete _ _ ct2 with "Hrmap") as "[Hct2 Hrmap]"; first by simplify_map_eq.
+    assert ( rmap' !! ct3 = Some (WInt 0) ) as Hwct3'.
+    { apply Hrmap_init'. rewrite Hdom_rmap'.
+      apply elem_of_difference; split; [apply all_registers_s_correct|set_solver].
+    }
+    iDestruct (big_sepM_delete _ _ ct3 with "Hrmap") as "[Hct3 Hrmap]"; first by simplify_map_eq.
+    assert ( rmap' !! ct4 = Some (WInt 0) ) as Hwct4'.
+    { apply Hrmap_init'. rewrite Hdom_rmap'.
+      apply elem_of_difference; split; [apply all_registers_s_correct|set_solver].
+    }
+    iDestruct (big_sepM_delete _ _ ct4 with "Hrmap") as "[Hct4 Hrmap]"; first by simplify_map_eq.
+    assert ( rmap' !! cs0 = Some (WInt 0) ) as Hwcs0'.
+    { apply Hrmap_init'. rewrite Hdom_rmap'.
+      apply elem_of_difference; split; [apply all_registers_s_correct|set_solver].
+    }
+    iDestruct (big_sepM_delete _ _ cs0 with "Hrmap") as "[Hcs0 Hrmap]"; first by simplify_map_eq.
+    assert ( rmap' !! cs1 = Some (WInt 0) ) as Hwcs1'.
+    { apply Hrmap_init'. rewrite Hdom_rmap'.
+      apply elem_of_difference; split; [apply all_registers_s_correct|set_solver].
+    }
+    iDestruct (big_sepM_delete _ _ cs1 with "Hrmap") as "[Hcs1 Hrmap]"; first by simplify_map_eq.
+
+    (* Load ct0 cgp  *)
+    iInstr "Hcode".
+    { split; [done| solve_addr]. }
+    (* Mov ct1 0  *)
+    iInstr "Hcode".
+    subst hcont; unfocus_block "Hcode" "Hcont" as "Hcode_main".
+
+    (* --------------------------------------------------- *)
+    (* ----------------- BLOCK 4: ASSERT ----------------- *)
+    (* --------------------------------------------------- *)
+
+    focus_block 4 "Hcode_main" as a_assert_c Ha_assert_c "Hcode" "Hcont"; iHide "Hcont" as hcont.
+    iApply (assert_success_spec with
+             "[- $Hassert $Hna $HPC $Hct2 $Hct3 $Hct4 $Hct0 $Hct1 $Hcra
+              $Hcode $Himport_assert]"); auto.
+    { solve_addr. }
+    iNext; iIntros "(Hna & HPC & Hct2 & Hct3 & Hct4 & Hcra & Hct0 & Hct1
+                    & Hcode & Himport_assert)".
+    subst hcont; unfocus_block "Hcode" "Hcont" as "Hcode_main".
+
+    (* --------------------------------------------------- *)
+    (* --------------- BLOCK 5: PREP CALL ---------------- *)
+    (* --------------------------------------------------- *)
+
+    set (cgp_c := (cgp_b ^+ 1)%a).
+    focus_block 5 "Hcode_main" as a_prepC Ha_prepC "Hcode" "Hcont"; iHide "Hcont" as hcont.
+    (* Mov ca0 cgp  *)
+    iInstr "Hcode".
+    (* Mov ca1 0  *)
+    iInstr "Hcode".
+    (* Lea cgp (-1)%Z *)
+    iInstr "Hcode".
+    { transitivity (Some cgp_b%a); auto; subst cgp_c; solve_addr. }
+
+    assert (std W2 B !! cgp_b = Some Permanent) as HW2_B_cpg_b.
+    { eapply monotone.region_state_pub_perm in HW1_pubB_W2; eauto.
+      subst W1.
+      (* TODO lemma *)
+      rewrite /std_update /std_update_cview /std /std_cview.
+      destruct (W_init_B !! B); rewrite !lookup_insert; done.
+    }
+    iDestruct (region_open with "[$Hrel_cgp_b $HWreg_B $HWstd_full_B]")
+      as (wcgp_b) "(HWreg_B & HWsts_full_B & HWstd_full_B & Hcpg_b & _ & HmonoR & #Hinterp_wcpgb)"
+    ; auto.
+    destruct (decide (Permanent = Temporary ∧ isWL RW = true)) as [ [? ?] | _ ]; first congruence.
+
+    (* Store cgp 42%Z *)
+    iInstr "Hcode".
+    { solve_addr. }
+
+    (* GetA ct0 ca0 *)
+    iInstr "Hcode".
+
+    (* Add ct1 ct0 1%Z *)
+    iInstr "Hcode".
+
+    (* Subseg ca0 ct0 ct1 *)
+    iInstr "Hcode".
+    { transitivity (Some (cgp_c ^+1)%a); auto; subst cgp_c; solve_addr. }
+    { subst cgp_c; solve_addr. }
+    subst hcont; unfocus_block "Hcode" "Hcont" as "Hcode_main".
+
+    (* --------------------------------------------------- *)
+    (* -------------- BLOCK 6 and 7: FETCH --------------- *)
+    (* --------------------------------------------------- *)
+
+    focus_block 6 "Hcode_main" as a_fetch3 Ha_fetch3 "Hcode" "Hcont"; iHide "Hcont" as hcont.
+    iApply (fetch_spec with "[- $HPC $Hctp $Hct0 $Hct1 $Hcode]"); eauto.
+    { solve_addr. }
+    replace (pc_b ^+ 0)%a with pc_b by solve_addr.
+    iFrame "Himport_switcher".
+    iNext ; iIntros "(HPC & Hctp & Hct0 & Hct1 & Hcode & Himport_switcher)".
+    iEval (cbn) in "Hctp".
+    subst hcont; unfocus_block "Hcode" "Hcont" as "Hcode_main".
+
+    focus_block 7 "Hcode_main" as a_fetch4 Ha_fetch4 "Hcode" "Hcont"; iHide "Hcont" as hcont.
+    iApply (fetch_spec with "[- $HPC $Hcs0 $Hct0 $Hct1 $Hcode $Himport_C_g]"); eauto.
+    { solve_addr. }
+    iNext ; iIntros "(HPC & Hcs0 & Hct0 & Hct1 & Hcode & Himport_C_g)".
+    iEval (cbn) in "Hcs0".
+    subst hcont; unfocus_block "Hcode" "Hcont" as "Hcode_main".
+
+    (* --------------------------------------------------- *)
+    (* ---------------- BLOCK 8: CALL C ------------------ *)
+    (* --------------------------------------------------- *)
+
+    focus_block 8 "Hcode_main" as a_callC Ha_callC "Hcode" "Hcont"; iHide "Hcont" as hcont.
+    iInstr "Hcode".
+
+    (* -- separate argument registers -- *)
+    assert ( rmap' !! ca2 = Some (WInt 0) ) as Hwca2'.
+    { apply Hrmap_init'. rewrite Hdom_rmap'.
+      apply elem_of_difference; split; [apply all_registers_s_correct|set_solver].
+    }
+    iDestruct (big_sepM_delete _ _ ca2 with "Hrmap") as "[Hca2 Hrmap]"; first by simplify_map_eq.
+    assert ( rmap' !! ca3 = Some (WInt 0) ) as Hwca3'.
+    { apply Hrmap_init'. rewrite Hdom_rmap'.
+      apply elem_of_difference; split; [apply all_registers_s_correct|set_solver].
+    }
+    iDestruct (big_sepM_delete _ _ ca3 with "Hrmap") as "[Hca3 Hrmap]"; first by simplify_map_eq.
+    assert ( rmap' !! ca4 = Some (WInt 0) ) as Hwca4'.
+    { apply Hrmap_init'. rewrite Hdom_rmap'.
+      apply elem_of_difference; split; [apply all_registers_s_correct|set_solver].
+    }
+    iDestruct (big_sepM_delete _ _ ca4 with "Hrmap") as "[Hca4 Hrmap]"; first by simplify_map_eq.
+    assert ( rmap' !! ca5 = Some (WInt 0) ) as Hwca5'.
+    { apply Hrmap_init'. rewrite Hdom_rmap'.
+      apply elem_of_difference; split; [apply all_registers_s_correct|set_solver].
+    }
+    iDestruct (big_sepM_delete _ _ ca5 with "Hrmap") as "[Hca5 Hrmap]"; first by simplify_map_eq.
+
+    subst rmap_arg.
+    set ( rmap_arg :=
+           {[ ca0 := WCap RW Global cgp_c%a (cgp_c ^+ 1)%a cgp_c%a;
+              ca1 := WInt 0;
+              ca2 := WInt 0;
+              ca3 := WInt 0;
+              ca4 := WInt 0;
+              ca5 := WInt 0;
+              ct0 := WInt 0
+           ]} : Reg
+        ).
+
+    rewrite !(delete_commute _ _ ct4).
+    iDestruct (big_sepM_insert _ _ ct4 with "[$Hrmap $Hct4]") as "Hrmap"; first by simplify_map_eq.
+    rewrite insert_delete_insert.
+    repeat (rewrite -delete_insert_ne //).
+    rewrite !(delete_commute _ _ ct3).
+    iDestruct (big_sepM_insert _ _ ct3 with "[$Hrmap $Hct3]") as "Hrmap"; first by simplify_map_eq.
+    rewrite insert_delete_insert.
+    repeat (rewrite -delete_insert_ne //).
+    rewrite !(delete_commute _ _ ct2).
+    iDestruct (big_sepM_insert _ _ ct2 with "[$Hrmap $Hct2]") as "Hrmap"; first by simplify_map_eq.
+    rewrite insert_delete_insert.
+    repeat (rewrite -delete_insert_ne //).
+    rewrite !(delete_commute _ _ ct1).
+    iDestruct (big_sepM_insert _ _ ct1 with "[$Hrmap $Hct1]") as "Hrmap"; first by simplify_map_eq.
+    rewrite insert_delete_insert.
+    repeat (rewrite -delete_insert_ne //).
+    rewrite !(delete_commute _ _ ctp).
+    iDestruct (big_sepM_insert _ _ ctp with "[$Hrmap $Hctp]") as "Hrmap"; first by simplify_map_eq.
+    rewrite insert_delete_insert.
+    repeat (rewrite -delete_insert_ne //).
+
+    set (rmap'' := (delete ca5 _)).
+
+    iMod (extend_region_perm _ _ _ _ _ RW interpC
+           with "[] [$HWstd_full_C] [$HWreg_C] [$Hcgp_c] []")
+      as "(HWreg_C & Hrel_cgp_c & HWstd_full_C)".
+    { done. }
+    { done. }
+    { iApply future_priv_mono_interp_z. }
+    { cbn; iEval (rewrite fixpoint_interp1_eq); done. }
+
+    set (W3 := <s[(C,cgp_c):=Permanent]s>W_init_C).
+    assert (related_sts_priv_world W_init_C W3 C) as HWinit_privC_W3.
+    { subst W3; by eapply related_sts_priv_world_fresh_Permanent. }
+
+    iAssert (interp W3 C (WSealed ot_switcher C_g)) as "#Hinterp_W3_C_g".
+    { iApply monotone.interp_monotone_sd; eauto. }
+
+    iAssert (interp W3 C (WCap RW Global cgp_c (cgp_c ^+ 1)%a cgp_c)) as "#Hinterp_W3_C_c".
+    { subst cgp_c.
+      iEval (cbn). iEval (rewrite fixpoint_interp1_eq). iEval (cbn).
+      rewrite finz_seq_between_cons; last solve_addr.
+      rewrite finz_seq_between_empty; last solve_addr.
+      iApply big_sepL_singleton.
+      iExists RW, interp.
+      iEval (cbn).
+      iSplit; first done.
+      iSplit; first (iPureIntro ; by apply persistent_cond_interp).
+      iSplit; first iFrame "Hrel_cgp_c".
+      iSplit; first (iNext ; by iApply zcond_interp).
+      iSplit; first (iNext ; by iApply rcond_interp).
+      iSplit; first (iNext ; by iApply wcond_interp).
+      subst W3.
+      iSplit.
+      + iApply monoReq_interp; last done.
+        rewrite /std_update /std_update_cview /std /std_cview.
+        destruct (W_init_C !! C); rewrite !lookup_insert; done.
+      + iPureIntro.
+        rewrite /std_update /std_update_cview /std /std_cview.
+        destruct (W_init_C !! C); rewrite !lookup_insert; done.
+    }
+
+    iAssert ([∗ map] rarg↦warg ∈ rmap_arg, rarg ↦ᵣ warg ∗ interp W3 C warg )%I
+      with "[Hca0 Hca1 Hca2 Hca3 Hca4 Hca5 Hct0]" as "Hrmap_arg".
+    { subst rmap_arg.
+      iAssert (interp W3 C (WInt 0)) as "Hinterp_0".
+      { iEval (rewrite fixpoint_interp1_eq); done. }
+      repeat (iApply big_sepM_insert; [done|iFrame "∗#"]).
+      done.
+    }
+
+    iApply (switcher_cc_specification _ _ W3 W3 with
+             "[- $Hswitcher $Hna
+              $HPC $Hcgp $Hcra $Hcsp $Hcs0 $Hcs1 $Hrmap_arg $Hrmap
+              $Hcsp_stk $HWreg_C $HWstd_full_C
+              $Hinterp_W3_C_g]"); auto.
+    { set_solver. }
+    { subst rmap''.
+      repeat (rewrite dom_delete_L); repeat (rewrite dom_insert_L).
+      rewrite Hdom_rmap'.
+      set_solver.
+    }
+    iSplitR.
+    { iIntros "(Hcsp_stk & HWreg_B & Hstd_full_B)". iModIntro; iFrame. }
+    iNext. subst rmap''.
+    iIntros "H".
+    iDestruct "H"
+      as (W4 rmap'') "(%HW1_pubB_W4 & %Hdom_rmap''
+                      & Hna & HWreg_C & HWstd_full_C
+                      & HPC & Hcgp & Hcra & Hcsp & Hca0 & Hca1
+                      & Hrmap & Hcsp_stk)".
+    iDestruct "Hca0" as (warg0') "[Hca0 _]".
+    iDestruct "Hca1" as (warg1') "[Hca1 _]".
+    rewrite updatePcPerm_seal_perm_sentry; last solve_pure.
+
+    iDestruct (big_sepM_sep with "Hrmap") as "[Hrmap Hrmap_zero]".
+    iDestruct (big_sepM_pure with "Hrmap_zero") as "%Hrmap_zero'".
+    assert (∀ r : RegName, r ∈ dom rmap'' → rmap'' !! r = Some (WInt 0)) as Hrmap_init''.
+    { intros r Hr.
+      rewrite elem_of_dom in Hr. destruct Hr as [wr Hr].
+      pose proof Hr as Hr'.
+      eapply map_Forall_lookup in Hr'; eauto.
+      by cbn in Hr' ; simplify_eq.
+    }
+    iClear "Hrmap_zero".
+
+    (* ---- extract the needed registers ctp ct0 ct1 ct2 ct3 ct4 cs0 ----  *)
+    assert ( rmap'' !! ctp = Some (WInt 0) ) as Hwctp''.
+    { apply Hrmap_init''. rewrite Hdom_rmap''.
+      apply elem_of_difference; split; [apply all_registers_s_correct|set_solver].
+    }
+    iDestruct (big_sepM_delete _ _ ctp with "Hrmap") as "[Hctp Hrmap]"; first by simplify_map_eq.
+    assert ( rmap'' !! ct0 = Some (WInt 0) ) as Hwct0''.
+    { apply Hrmap_init''. rewrite Hdom_rmap''.
+      apply elem_of_difference; split; [apply all_registers_s_correct|set_solver].
+    }
+    iDestruct (big_sepM_delete _ _ ct0 with "Hrmap") as "[Hct0 Hrmap]"; first by simplify_map_eq.
+    assert ( rmap'' !! ct1 = Some (WInt 0) ) as Hwct1''.
+    { apply Hrmap_init''. rewrite Hdom_rmap''.
+      apply elem_of_difference; split; [apply all_registers_s_correct|set_solver].
+    }
+    iDestruct (big_sepM_delete _ _ ct1 with "Hrmap") as "[Hct1 Hrmap]"; first by simplify_map_eq.
+    assert ( rmap'' !! ct2 = Some (WInt 0) ) as Hwct2''.
+    { apply Hrmap_init''. rewrite Hdom_rmap''.
+      apply elem_of_difference; split; [apply all_registers_s_correct|set_solver].
+    }
+    iDestruct (big_sepM_delete _ _ ct2 with "Hrmap") as "[Hct2 Hrmap]"; first by simplify_map_eq.
+    assert ( rmap'' !! ct3 = Some (WInt 0) ) as Hwct3''.
+    { apply Hrmap_init''. rewrite Hdom_rmap''.
+      apply elem_of_difference; split; [apply all_registers_s_correct|set_solver].
+    }
+    iDestruct (big_sepM_delete _ _ ct3 with "Hrmap") as "[Hct3 Hrmap]"; first by simplify_map_eq.
+    assert ( rmap'' !! ct4 = Some (WInt 0) ) as Hwct4''.
+    { apply Hrmap_init''. rewrite Hdom_rmap''.
+      apply elem_of_difference; split; [apply all_registers_s_correct|set_solver].
+    }
+    iDestruct (big_sepM_delete _ _ ct4 with "Hrmap") as "[Hct4 Hrmap]"; first by simplify_map_eq.
+    assert ( rmap'' !! cs0 = Some (WInt 0) ) as Hwcs0''.
+    { apply Hrmap_init''. rewrite Hdom_rmap''.
+      apply elem_of_difference; split; [apply all_registers_s_correct|set_solver].
+    }
+    iDestruct (big_sepM_delete _ _ cs0 with "Hrmap") as "[Hcs0 Hrmap]"; first by simplify_map_eq.
+    assert ( rmap'' !! cs1 = Some (WInt 0) ) as Hwcs1''.
+    { apply Hrmap_init''. rewrite Hdom_rmap''.
+      apply elem_of_difference; split; [apply all_registers_s_correct|set_solver].
+    }
+    iDestruct (big_sepM_delete _ _ cs1 with "Hrmap") as "[Hcs1 Hrmap]"; first by simplify_map_eq.
+
+    (* Load ct0 cgp  *)
+    iInstr "Hcode".
+    { split; [done| solve_addr]. }
+    (* Mov ct1 42  *)
+    iInstr "Hcode".
+    subst hcont; unfocus_block "Hcode" "Hcont" as "Hcode_main".
+
+    (* --------------------------------------------------- *)
+    (* ----------------- BLOCK 9: ASSERT ----------------- *)
+    (* --------------------------------------------------- *)
+
+    focus_block 9 "Hcode_main" as a_assert_b Ha_assert_b "Hcode" "Hcont"; iHide "Hcont" as hcont.
+    iApply (assert_success_spec with
+             "[- $Hassert $Hna $HPC $Hct2 $Hct3 $Hct4 $Hcra $Hct0 $Hct1
+              $Hcode $Himport_assert]"); auto.
+    { solve_addr. }
+    iNext; iIntros "(Hna & HPC & Hct2 & Hct3 & Hct4 & Hcra & Hct0 & Hct1
+                    & Hcode & Himport_assert)".
+    subst hcont; unfocus_block "Hcode" "Hcont" as "Hcode_main".
+
+    (* --------------------------------------------------- *)
+    (* ----------------- BLOCK 10: HALT ------------------ *)
+    (* --------------------------------------------------- *)
+
+    focus_block 10 "Hcode_main" as a_halt Ha_halt "Hcode" "Hcont"; iHide "Hcont" as hcont.
+    iInstr "Hcode".
+    subst hcont; unfocus_block "Hcode" "Hcont" as "Hcode_main".
+
+    subst hφ; iApply ("Hφ" with "[$]").
+  Qed.
+
+  Lemma cmdc_spec_full
+
+    (pc_b pc_e pc_a : Addr)
+    (cgp_b cgp_e : Addr)
+    (csp_b csp_e : Addr)
+    (rmap : Reg)
+
+    (b_switcher e_switcher a_cc_switcher : Addr) (ot_switcher : OType)
+    (b_assert e_assert : Addr) (a_flag : Addr)
+    (B_f C_g : Sealable)
+
+    (W_init_B : WORLD)
+    (W_init_C : WORLD)
+
+    (csp_content : list Word)
+
+    (φ : language.val cap_lang -> iProp Σ)
+    (Nassert Nswitcher : namespace)
+    (E : coPset)
+    :
+
+    let imports :=
+     cmdc_main_imports b_switcher e_switcher a_cc_switcher ot_switcher b_assert e_assert B_f C_g
+    in
+
+    ↑Nswitcher ⊆ E ->
+    ↑Nassert ⊆ E ->
+
+    dom rmap = all_registers_s ∖ {[ PC ; cgp ; csp]} ->
+    (forall r, r ∈ dom rmap -> rmap !! r = Some (WInt 0) ) ->
+    SubBounds pc_b pc_e pc_a (pc_a ^+ length cmdc_main_code)%a ->
+
+    (cgp_b + length cmdc_main_data)%a = Some cgp_e ->
+    (pc_b + length imports)%a = Some pc_a ->
+
+    cgp_b ∉ dom (std W_init_B B) ->
+    (cgp_b ^+ 1)%a ∉ dom (std W_init_C C) ->
+
+    length csp_content = finz.dist csp_b csp_e ->
+
+    (
+      na_inv logrel_nais Nassert (assert_inv b_assert e_assert a_flag)
+      ∗ na_inv logrel_nais Nswitcher (switcher_inv b_switcher e_switcher a_cc_switcher ot_switcher)
+      ∗ na_own logrel_nais E
+
+      (* initial register file *)
+      ∗ PC ↦ᵣ WCap RX Global pc_b pc_e pc_a
+      ∗ cgp ↦ᵣ WCap RW Global cgp_b cgp_e cgp_b
+      ∗ csp ↦ᵣ WCap RWL Local csp_b csp_e csp_b
+      ∗ ( [∗ map] r↦w ∈ rmap, r ↦ᵣ w )
+
+      (* initial memory layout *)
+      ∗ [[ pc_b , pc_a ]] ↦ₐ [[ imports ]]
+      ∗ codefrag pc_a cmdc_main_code
+      ∗ [[ cgp_b , cgp_e ]] ↦ₐ [[ cmdc_main_data ]]
+      ∗ [[ csp_b , csp_e ]] ↦ₐ [[ csp_content ]]
+
+      ∗ region W_init_B B ∗ sts_full_world W_init_B B
+      ∗ region W_init_C C ∗ sts_full_world W_init_C C
+
+      ∗ interp W_init_B B (WSealed ot_switcher B_f)
+      ∗ interp W_init_C C (WSealed ot_switcher C_g)
+
+      ∗ ▷ (
+            na_own logrel_nais E
+              -∗ WP Instr Halted {{ λ v, φ v ∨ ⌜v = FailedV⌝ }})
+      ⊢ WP Seq (Instr Executable) {{ λ v, True }})%I.
+  Proof.
+    intros imports; subst imports.
+    iIntros (HNswitcherE HNassertE Hrmap_dom Hrmap_init HsubBounds
+               Hcgp_contiguous Himports_contiguous Hcgp_b Hcgp_c Hlen_stack)
+      "(#Hassert & #Hswitcher & Hna
+      & HPC & Hcgp & Hcsp & Hrmap
+      & Himports_main & Hcode_main & Hcgp_main & Hcsp_stk
+      & HWreg_B & HWstd_full_B
+      & HWreg_C & HWstd_full_C
+      & #Hinterp_Winit_B_f & #Hinterp_Winit_C_g
+      & Hφ)".
+    iApply (wp_wand with "[-]").
+    { iApply (cmdc_spec
+                pc_b pc_e pc_a cgp_b cgp_e csp_b csp_e rmap
+                b_switcher e_switcher a_cc_switcher ot_switcher
+                b_assert e_assert a_flag B_f C_g W_init_B W_init_C
+                csp_content φ Nassert Nswitcher E); eauto; iFrame "#∗".
+    }
+    by iIntros (v) "?".
+  Qed.
+
+End CMDC.
